Semantics

Program_Logic.thy
@@ -1,6 +1,7 @@
 theory Program_Logic
 
-imports Invalid_Ops
+imports  MMU_ARM
+        
 
 begin               
 
@@ -31,56 +32,60 @@ datatype com =  SKIP
              |  If bexp com com       ("(IF _/ THEN _/ ELSE _)"  [0, 0, 61] 61)
              |  While bexp com        ("(WHILE _/ DO _)"  [0, 61] 61)
 
+definition "K1 \<equiv> \<lambda>x y. (x , y)"
+
+definition
+  "oreturn1 = K1 o Some"
+
+definition
+  "ofail1 = K1  None"
 
 
-
-   (* Semantics *)
 
 fun aval :: "aexp \<Rightarrow> 'a::mem_op state_scheme \<Rightarrow> val option \<times> 'a state_scheme " where
-"aval (Const c)  = return (Some c)" |
+"aval (Const c)  = oreturn1 c" |
 "aval (BinOp f e1 e2) = do {
                            avale1 <- aval e1;
                            avale2 <- aval e2;
-                           case (avale1  , avale2) of (Some v1 , Some v2) \<Rightarrow> return (Some (f v1 v2)) |
-                                 _ \<Rightarrow> return (None) }" |
+                           case (avale1 , avale2) of (Some v1 , Some v2) \<Rightarrow> oreturn1 (f v1 v2) |
+                                 _ \<Rightarrow> ofail1  }" |
 "aval (UnOp f e) = do {
                            avale <- aval e;
-                           case avale of Some v \<Rightarrow> return (Some (f v)) |
-                                 _ \<Rightarrow> return (None) }" |
+                           case avale of Some v \<Rightarrow> oreturn1 (f v) |
+                                 _ \<Rightarrow> ofail1 }" |
 "aval (HeapLookup vp)  = do { 
                             avalvp <- aval vp; 
-                            case avalvp of None \<Rightarrow> return None  | Some v \<Rightarrow> 
+                            case avalvp of None \<Rightarrow> ofail1 | 
+                               Some v \<Rightarrow> 
                                do {
                                    bl <-  mmu_read_size (Addr v , 4);
                                    exp <- read_state exception;
                                    if exp = NoException 
                                    then do {
-                                      return  
-                                        (Some (of_bl (bitstring_field 31 0 bl)))
+                                      oreturn1 (of_bl (bitstring_field 31 0 bl))
                                         }
-                                   else return None
+                                   else ofail1
                                 }
                               }"
 
 
 
 fun bval :: "bexp \<Rightarrow> 'a::mem_op state_scheme \<Rightarrow> bool option \<times> 'a state_scheme" where
-"bval (BConst b)  = return (Some b)" |
+"bval (BConst b)  = oreturn1 b" |
 "bval (BComp f e1 e2) = do {
                            v1 <- aval e1;
                            v2 <- aval e2;
-                           case (v1  , v2) of (Some v1 , Some v2) \<Rightarrow> return (Some (f v1 v2)) |
-                                 _ \<Rightarrow> return (None) }" |
+                           case (v1  , v2) of (Some v1 , Some v2) \<Rightarrow> oreturn1 (f v1 v2) |
+                                 _ \<Rightarrow> ofail1 }" |
 "bval (BBinOp f b1 b2) = do {
                            bvale1 <- bval b1;
                            bvale2 <- bval b2;
-                           case (bvale1  , bvale2) of (Some v1 , Some v2) \<Rightarrow> return (Some (f v1 v2)) |
-                                 _ \<Rightarrow> return (None) }"|
+                           case (bvale1  , bvale2) of (Some v1 , Some v2) \<Rightarrow> oreturn1 (f v1 v2) |
+                                 _ \<Rightarrow> ofail1 }"|
 "bval (BNot b)  = do { 
                           bvale <- bval b;
-                          case bvale of Some v \<Rightarrow> return (Some (\<not>v)) |
-                                 _ \<Rightarrow> return (None) }"
-
+                          case bvale of Some v \<Rightarrow> oreturn1  (\<not>v) |
+                                 _ \<Rightarrow> ofail1 }"
 
 
 inductive
@@ -88,7 +93,8 @@ inductive
 where
 Skip:       "(SKIP,s) \<Rightarrow> Some s"   |
 AssignFail: "\<lbrakk>aval lval s = (None, _) \<or> aval rval s = (None, _) \<rbrakk>  \<Longrightarrow> (lval ::= rval , s) \<Rightarrow> None" |
-Assign:     "\<lbrakk>aval lval s = (Some vp, _) ; aval rval s = (Some v, _) \<rbrakk>  \<Longrightarrow> (lval ::= rval , s) \<Rightarrow> None"|
+Assign:     "\<lbrakk>aval lval s = (Some vp, _) ; aval rval s = (Some v, _) \<rbrakk>  \<Longrightarrow> (lval ::= rval , s) \<Rightarrow> 
+              Some (snd (mmu_write_size (to_bl v, (Addr vp), 4) s) )"|
 Seq:        "\<lbrakk>(c1,s1) \<Rightarrow> Some s2;  (c2,s2) \<Rightarrow> s3 \<rbrakk> \<Longrightarrow> (c1;;c2, s1) \<Rightarrow> s3" |
 SeqFail:    "(c1,s1) \<Rightarrow> None \<Longrightarrow> (c1;;c2, s1) \<Rightarrow> None" |
 IfTrue:     "\<lbrakk>bval b s = (Some True, _); (c1,s) \<Rightarrow> t \<rbrakk> \<Longrightarrow> (IF b THEN c1 ELSE c2, s) \<Rightarrow> t" |
@@ -99,7 +105,8 @@ WhileTrue:  "\<lbrakk>bval b s = (Some True, _) ; (c, s) \<Rightarrow> Some s'';
 WhileFail1: "\<lbrakk>bval b s = (Some True, _) ; (c, s) \<Rightarrow> None \<rbrakk>\<Longrightarrow> (WHILE b DO c , s) \<Rightarrow> None" |
 WhileFail2: "bval b s = (None, _) \<Longrightarrow> (WHILE b DO c , s) \<Rightarrow> None" 
 
-
+code_pred big_step .
+declare big_step.intros [intro]
 thm big_step.induct
 lemmas big_step_induct = big_step.induct [split_format (complete)]
 thm big_step_induct
@@ -119,42 +126,49 @@ thm SkipE
     
 
 
-(*type_synonym assn = "state \<Rightarrow> bool" *)
-
 definition
   hoare_valid :: "('a::mem_op state_scheme \<Rightarrow> bool) \<Rightarrow> com \<Rightarrow> ('a::mem_op state_scheme \<Rightarrow> bool) \<Rightarrow> bool" ("\<Turnstile> \<lbrace>(1_)\<rbrace>/ (_)/ \<lbrace>(1_)\<rbrace>" 50) where
   "\<Turnstile> \<lbrace>P\<rbrace> c \<lbrace>Q1\<rbrace> \<equiv> \<forall>s s'. (c,s) \<Rightarrow> s' \<and> P s \<longrightarrow> (\<exists>r. s' = Some r \<and> Q1 r)"
+
 
 lemma skip_sound:
   "\<Turnstile> \<lbrace>P\<rbrace> SKIP \<lbrace>P\<rbrace>"
   by (clarsimp simp: hoare_valid_def)
 
+lemma  assign_sound:
+  " \<Turnstile> \<lbrace>\<lambda>s. P (snd (mmu_write_size (to_bl (the (fst (aval r s))), Addr (the (fst (aval l s))), 4) s)) \<and>
+       fst (aval l s)  \<noteq> None \<and> fst (aval r s)  \<noteq> None \<rbrace>  l ::= r \<lbrace>P\<rbrace>" 
+  apply (clarsimp simp: hoare_valid_def)
+  apply auto
+  done
+
+
 lemma seq_sound:
-  "\<lbrakk> \<Turnstile> \<lbrace>P\<rbrace> c1 \<lbrace>Q1\<rbrace> \<and> \<Turnstile> \<lbrace>Q1\<rbrace> c2 \<lbrace>R1\<rbrace> \<rbrakk>  \<Longrightarrow> \<Turnstile> \<lbrace>P\<rbrace> c1;;c2 \<lbrace>R1\<rbrace>"
+  "\<lbrakk> \<Turnstile> \<lbrace>P\<rbrace> c1 \<lbrace>QQ\<rbrace> ; \<Turnstile> \<lbrace>QQ\<rbrace> c2 \<lbrace>R1\<rbrace> \<rbrakk>  \<Longrightarrow> \<Turnstile> \<lbrace>P\<rbrace> c1;;c2 \<lbrace>R1\<rbrace>"
   apply (clarsimp simp: hoare_valid_def)
   by blast
 
 
 lemma conseq_sound:
-  "\<lbrakk> \<Turnstile> \<lbrace>P\<rbrace> c \<lbrace>Q1\<rbrace> \<and> (\<forall>s. P' s \<longrightarrow> P s) \<and> (\<forall>s. Q1 s \<longrightarrow> Q' s) \<rbrakk>  
+  "\<lbrakk> \<Turnstile> \<lbrace>P\<rbrace> c \<lbrace>Q1\<rbrace> ; (\<forall>s. P' s \<longrightarrow> P s) \<and> (\<forall>s. Q1 s \<longrightarrow> Q' s) \<rbrakk>  
          \<Longrightarrow> \<Turnstile> \<lbrace>P'\<rbrace> c \<lbrace>Q'\<rbrace>"
   apply (clarsimp simp: hoare_valid_def)
   by blast
 
 lemma conj_sound:
-  "\<lbrakk> \<Turnstile> \<lbrace>P\<rbrace> c \<lbrace>Q1\<rbrace> \<and> \<Turnstile> \<lbrace>R1\<rbrace> c \<lbrace>S1\<rbrace> \<rbrakk>  \<Longrightarrow> \<Turnstile> \<lbrace>\<lambda>s. P s \<and> R1 s\<rbrace> c \<lbrace>\<lambda>s. Q1 s \<and> S1 s\<rbrace>"
+  "\<lbrakk> \<Turnstile> \<lbrace>P\<rbrace> c \<lbrace>Q1\<rbrace> ; \<Turnstile> \<lbrace>R1\<rbrace> c \<lbrace>S1\<rbrace> \<rbrakk>  \<Longrightarrow> \<Turnstile> \<lbrace>\<lambda>s. P s \<and> R1 s\<rbrace> c \<lbrace>\<lambda>s. Q1 s \<and> S1 s\<rbrace>"
   apply (clarsimp simp: hoare_valid_def)
   by blast
 
 
 lemma disj_sound:
-  "\<lbrakk> \<Turnstile> \<lbrace>P\<rbrace> c \<lbrace>Q1\<rbrace> \<and> \<Turnstile> \<lbrace>R1\<rbrace> c \<lbrace>S1\<rbrace> \<rbrakk>  \<Longrightarrow> \<Turnstile> \<lbrace>\<lambda>s. P s \<or> R1 s\<rbrace> c \<lbrace>\<lambda>s. Q1 s \<or> S1 s\<rbrace>"
+  "\<lbrakk> \<Turnstile> \<lbrace>P\<rbrace> c \<lbrace>Q1\<rbrace> ; \<Turnstile> \<lbrace>R1\<rbrace> c \<lbrace>S1\<rbrace> \<rbrakk>  \<Longrightarrow> \<Turnstile> \<lbrace>\<lambda>s. P s \<or> R1 s\<rbrace> c \<lbrace>\<lambda>s. Q1 s \<or> S1 s\<rbrace>"
   apply (clarsimp simp: hoare_valid_def)
   by blast
 
 
 lemma if_sound:
-  "\<lbrakk> \<Turnstile> \<lbrace>\<lambda>s. P s \<and> fst (bval b s) = Some True \<rbrace> c1 \<lbrace>Q1\<rbrace> \<and> 
+  "\<lbrakk> \<Turnstile> \<lbrace>\<lambda>s. P s \<and> fst (bval b s) = Some True \<rbrace> c1 \<lbrace>Q1\<rbrace> ; 
      \<Turnstile> \<lbrace>\<lambda>s. P s \<and> fst (bval b s) = Some False\<rbrace> c2 \<lbrace>Q1\<rbrace> \<rbrakk>  \<Longrightarrow>
         \<Turnstile> \<lbrace>\<lambda>s. P s \<and> fst (bval b s) \<noteq> None\<rbrace> IF b THEN c1 ELSE c2 \<lbrace>Q1\<rbrace>"
   apply (clarsimp simp:  hoare_valid_def)
@@ -170,7 +184,7 @@ lemma while_final:
   done
 
 lemma while_sound:
-  "\<lbrakk> \<Turnstile> \<lbrace>\<lambda>s. P s \<and> fst (bval b s) = Some True \<rbrace> c \<lbrace>P\<rbrace> \<and> 
+  "\<lbrakk> \<Turnstile> \<lbrace>\<lambda>s. P s \<and> fst (bval b s) = Some True \<rbrace> c \<lbrace>P\<rbrace> ;
         (\<forall>s. P s \<longrightarrow> fst (bval b s) \<noteq> None) \<rbrakk>  \<Longrightarrow>
         \<Turnstile> \<lbrace>P\<rbrace> WHILE b DO c \<lbrace>\<lambda>s. P s \<and> fst (bval b s) = Some False\<rbrace>"
   apply (clarsimp simp:  hoare_valid_def)
@@ -179,21 +193,76 @@ lemma while_sound:
      apply(rule_tac c = c and s'' = s'' in while_final) apply fastforce +
 done
 
-print_theorems 
 
-(* Assign Sound *)
-lemma 
-  "\<Turnstile> \<lbrace>P\<rbrace> l ::= r \<lbrace>P\<rbrace>" (* remaining *)
+(*  -----------------------  *)
+
+(*
+lemma skip_sound1:
+  "\<Turnstile> \<lbrace>P\<rbrace> SKIP \<lbrace>P\<rbrace>"
+  by (clarsimp simp: hoare_valid_def)
+
+lemma  assign_sound1:
+  " \<Turnstile> \<lbrace>\<lambda>s. P (snd (mmu_write_size (to_bl (the (fst (aval r s))), Addr (the (fst (aval l s))), 4) s)) \<and>
+       fst (aval l s)  \<noteq> None \<and> fst (aval r s)  \<noteq> None \<rbrace>  l ::= r \<lbrace>P\<rbrace>" 
   apply (clarsimp simp: hoare_valid_def)
+  apply auto
+  done
 
-oops
+
+lemma seq_sound1:
+  "\<lbrakk> \<Turnstile> \<lbrace>P\<rbrace> c1 \<lbrace>Q1\<rbrace> ; \<Turnstile> \<lbrace>Q1\<rbrace> c2 \<lbrace>R1\<rbrace> \<rbrakk>  \<Longrightarrow> \<Turnstile> \<lbrace>P\<rbrace> c1;;c2 \<lbrace>R1\<rbrace>"
+  apply (clarsimp simp: hoare_valid_def)
+  by blast
 
 
+lemma conseq_sound1:
+  "\<lbrakk> \<Turnstile> \<lbrace>P'\<rbrace> c \<lbrace>Q'\<rbrace> ; (\<forall>s. P1 s \<longrightarrow> P' s) \<and> (\<forall>s. Q' s \<longrightarrow> Q1 s) \<rbrakk>  
+         \<Longrightarrow> \<Turnstile> \<lbrace>P1\<rbrace> c \<lbrace>Q1\<rbrace>"
+  apply (clarsimp simp: hoare_valid_def)
+  by blast
 
-declare [[show_types]]
+lemma conj_sound1:
+  "\<lbrakk> \<Turnstile> \<lbrace>P\<rbrace> c \<lbrace>Q1\<rbrace> ; \<Turnstile> \<lbrace>R1\<rbrace> c \<lbrace>S1\<rbrace> \<rbrakk>  \<Longrightarrow> 
+   \<Turnstile> \<lbrace>\<lambda>s. P s \<and> R1 s\<rbrace> c \<lbrace>\<lambda>s. Q1 s \<and> S1 s\<rbrace>"
+  apply (clarsimp simp: hoare_valid_def)
+  by blast
 
-thm Run_def
 
-thm DecodeARM_def
+lemma disj_sound1:
+  "\<lbrakk> \<Turnstile> \<lbrace>P\<rbrace> c \<lbrace>Q1\<rbrace> ; \<Turnstile> \<lbrace>R1\<rbrace> c \<lbrace>S1\<rbrace> \<rbrakk>  \<Longrightarrow> \<Turnstile> \<lbrace>\<lambda>s. P s \<or> R1 s\<rbrace> c \<lbrace>\<lambda>s. Q1 s \<or> S1 s\<rbrace>"
+  apply (clarsimp simp: hoare_valid_def)
+  by blast
 
+
+lemma if_sound1:
+  "\<lbrakk> \<Turnstile> \<lbrace>\<lambda>s. P s \<and> fst (bval b s) = Some True \<rbrace> c1 \<lbrace>Q1\<rbrace> ; 
+     \<Turnstile> \<lbrace>\<lambda>s. P s \<and> fst (bval b s) = Some False\<rbrace> c2 \<lbrace>Q1\<rbrace> \<rbrakk>  \<Longrightarrow>
+        \<Turnstile> \<lbrace>\<lambda>s. P s \<and> fst (bval b s) \<noteq> None\<rbrace> IF b THEN c1 ELSE c2 \<lbrace>Q1\<rbrace>"
+  apply (clarsimp simp:  hoare_valid_def)
+  by fastforce
+ 
+lemma while_final1:
+  "\<lbrakk>(prog, s'') \<Rightarrow> s';  
+     \<forall>s. P s \<and> fst (bval b s) = Some True \<longrightarrow> (\<forall>s'. (c, s) \<Rightarrow> s' \<longrightarrow> (\<exists>r. s' = Some r \<and> P r));  P s'';
+       \<forall>s. P s \<longrightarrow> (\<exists>y. fst (bval b s) = Some y); prog = WHILE b DO c \<rbrakk>  \<Longrightarrow> 
+        \<exists>r. s' = Some r \<and> P r \<and> fst (bval b r) = Some False"
+  apply(induct rule: big_step_induct)
+  apply fastforce+
+  done
+
+lemma while_sound1:
+  "\<lbrakk> \<Turnstile> \<lbrace>\<lambda>s. P s \<and> fst (bval b s) = Some True \<rbrace> c \<lbrace>P\<rbrace> ;
+        (\<forall>s. P s \<longrightarrow> fst (bval b s) \<noteq> None) \<rbrakk>  \<Longrightarrow>
+        \<Turnstile> \<lbrace>P\<rbrace> WHILE b DO c \<lbrace>\<lambda>s. P s \<and> fst (bval b s) = Some False\<rbrace>"
+  apply (clarsimp simp:  hoare_valid_def)
+  apply (erule WhileE)
+     prefer 2
+     apply(rule_tac c = c and s'' = s'' in while_final) apply fastforce +
+done
+
+
+(*   ---------------------- *)
+
+*)
 end
+
